theories/modules/FSpec.v
@@ -191,10 +191,10 @@ End fspec.
 Section fspec_WINV.
   Context `{!crisG Γ Σ α β τ _S _I}.
 
-  (* Definition fspec_winv (E : coPset) (fsp : fspec) : fspec :=
+  Definition fspec_winv (fsp : fspec) : fspec :=
     fspec_mk (meta := meta fsp)
-      (λ '(NS, tid) x varg arg, winv (E, E) ∗ precond fsp (NS, tid) x varg arg)%I
-      (λ '(NS, tid) x vret ret, winv (E, E) ∗ postcond fsp (NS, tid) x vret ret)%I. *)
+      (λ '(N, stid) x varg arg, winv (↑N, ↑N) ∗ precond fsp (N, stid) x varg arg)%I
+      (λ '(N, stid) x vret ret, winv (↑N, ↑N) ∗ postcond fsp (N, stid) x vret ret)%I.
 
   Definition icond_winv (E : coPset) (I : iProp Σ) : iProp Σ :=
     winv (E, E) ∗ I.
